SP1Chips.lean
@@ -1,5 +1,4 @@
 import SP1Chips.AddChip
-import SP1Chips.SubChip
 import SP1Chips.BitwiseChip
 import SP1Chips.JalChip
-import SP1Chips.XorChip
+import SP1Chips.SubChip
